coq-DataRF/PrimitivesFTyping222.v
@@ -1,0 +1,147 @@
+Require Import SystemRF.BasicDefinitions.
+Require Import SystemRF.Names.
+Require Import SystemRF.Semantics.
+Require Import SystemRF.SystemFWellFormedness.
+Require Import SystemRF.SystemFTyping.           
+
+(* -- | Well Formedness of System F PRIMITIVES *)
+
+Lemma lem_wfft_erase_ty : forall (g:fenv) (ds:defs) (c:prim),  
+    WFFT g ds (erase_ty c) Star.
+Proof. intros. destruct c; try (apply WFFTPoly with Star (bindsF g))
+                         ; intros; unfold unbindFT; simpl
+                         ; try (apply WFFTFunc with Base Star)
+                         ; try (apply WFFTFunc with Base Base)
+                         ; try (apply WFFTFV)
+                         ; try (apply WFFTKind)
+                         ; try (apply WFFTBasic)
+                         ; simpl; intuition. Qed.
+
+(*-----------------------------------------------------------------------------
+-- | (System F) TYPES of DELTA (of Applications of primitives)
+-----------------------------------------------------------------------------*)
+
+Definition isBool (e:expr) : Prop :=
+    match e with
+    | (Bc _ ) => True
+    | _       => False
+    end.
+
+Lemma lem_bool_values : forall (ds:defs) (v:expr), 
+    isValue v -> HasFtype FEmpty ds v (FTBasic TBool) ->  isBool v.
+Proof. intros ds v val p_v_bl. inversion p_v_bl; subst v;
+    (*try (inversion val; inversion H3).*)
+    try contradiction.
+    - (* v = Bc *) simpl; trivial.
+    - (* v = Prim *) destruct c; simpl in H3; discriminate.
+    - (* DC *) inversion val; try inversion H2. (* impossible somehow *)
+    - (* App *)
+    - (* AppT *)
+    - (* Let *)
+    - (* Annot *)
+    - (* Switch *)
+    Qed. 
+
+Definition isInt (e:expr) : Prop :=
+    match e with
+    | (Ic _ ) => True
+    | _       => False
+    end.
+
+Lemma lem_int_values : forall (v:expr),
+    isValue v -> HasFtype FEmpty v (FTBasic TInt) -> isInt v.
+Proof. intros v val p_v_Z. inversion p_v_Z; subst v; 
+    simpl in val; try contradiction.
+    - (* v = Ic *) auto.
+    - (* v = Prim *) destruct c; simpl in H2; discriminate.
+    Qed. 
+
+Definition isLambdaOrPrim (e:expr) : Prop :=
+    match e with
+    | (Prim _)   => True
+    | (Lambda _) => True
+    | _          => False
+    end.
+
+Definition isLambdaTOrPrim (e:expr) : Prop :=
+    match e with
+    | (Prim _)      => True
+    | (LambdaT _ _) => True
+    | _             => False
+    end.
+
+Definition isPoly (c:prim) : Prop :=
+    match c with
+    | Eql     => True
+    | Leql    => True
+    | _       => False
+    end.
+
+Lemma lemma_function_values : forall (v:expr) (t:ftype) (t':ftype),
+    isValue v -> HasFtype FEmpty v (FTFunc t t') -> isLambdaOrPrim v.
+Proof.  intros v t t' val p_v_tt'; inversion p_v_tt'; subst v;
+  simpl in val; try contradiction; auto. Qed.    
+
+Lemma lemma_tfunction_values : forall (v:expr) (k:kind) (t:ftype),
+    isValue v -> HasFtype FEmpty v (FTPoly k t) -> isLambdaTOrPrim v.
+Proof. intros v k t val p_v_kt; inversion p_v_kt; subst v;
+  simpl in val; try contradiction; auto. Qed.
+
+Lemma lem_prim_compat_in_ftapp : forall (p:prim) (v:expr) (t:ftype),
+    isValue v -> HasFtype FEmpty (App (Prim p) v) t -> isCompat' p v.
+Proof. intros p v t val p_pv_t. 
+  destruct p; inversion p_pv_t; inversion H2; subst b;
+  (apply lem_bool_values || apply lem_int_values); assumption. Qed.
+
+Lemma lem_delta_ftyp : forall (c:prim) (v:expr) (t_x:ftype) (t':ftype),
+    isValue v -> HasFtype FEmpty (Prim c) (FTFunc t_x t') -> HasFtype FEmpty v t_x
+              -> exists e, Some e = delta' c v /\ HasFtype FEmpty e t'.
+Proof. intros c v t_x t' val p_c_txt' p_v_tx. 
+  destruct c; inversion p_c_txt'; subst t_x;
+  try (apply (lem_bool_values v val) in p_v_tx as Hv);
+  try (apply (lem_int_values v val) in p_v_tx as Hv);
+  destruct v; try contradiction;
+  try (destruct b); simpl;
+  ( match goal with
+    | [ |- exists _, Some _ = Some ?term /\ _ ] => exists term
+    end )
+         ; split    
+         ; try (apply FTAbs with Base empty)
+         ; intros; unfold unbind; simpl
+         ; try (apply FTApp with (FTBasic TBool))
+         ; try (apply WFFTBasic)
+         ; try (apply FTVar)
+         ; try (apply FTPrm)
+         ; try (apply FTBC)
+         ; simpl; auto.
+  Qed.
+
+Lemma lem_base_types : forall (t:ftype),
+    WFFT FEmpty t Base -> isClosedBaseF t.
+Proof. intros t p_t_b; inversion p_t_b; subst t;
+  try (destruct b); simpl; simpl in H;
+  (trivial || contradiction). Qed.
+
+Lemma lem_prim_compatT_in_ftappt : forall (c:prim) (rt:type) (t:ftype),
+    HasFtype FEmpty (AppT (Prim c) rt) t  ->  isCompatT' c rt.
+Proof. intros c rt t p_crt_t. destruct c; inversion p_crt_t; inversion H1;
+  subst k; apply lem_base_types in H8; 
+  destruct (erase rt) eqn:Hrt; simpl in H8; try contradiction; 
+  simpl; rewrite Hrt; trivial. Qed.
+  
+Lemma lem_deltaT_ftyp : forall (c:prim) (k:kind) (s:ftype) (t:type),
+    HasFtype FEmpty (Prim c) (FTPoly k s) -> WFFT FEmpty (erase t) k
+        -> exists e, Some e = deltaT' c t /\ HasFtype FEmpty e (ftsubBV (erase t) s).
+Proof. intros c k s t p_c_aks p_emp_t; 
+  destruct c; inversion p_c_aks; subst k;
+  apply lem_base_types in p_emp_t as Ht;
+  destruct (erase t) eqn:E; try contradiction;
+  destruct b; try contradiction;
+  unfold deltaT'; rewrite E;
+  ( match goal with
+    | [ |- exists _, Some _ = Some ?term /\ _ ] => exists term
+    end )
+         ; split
+         ; try (apply FTPrm)
+         ; auto.
+  Qed.
